physical/CachedCPU_RV64IMAFD_Zicsr_Zifencei_Microcoded_synth.sv
@@ -6,6 +6,7 @@
 module CachedCPU_RV64IMAFD_Zicsr_Zifencei_Microcoded_synth (
   input  logic          clock,
   input  logic          reset,
+  input  logic          mtip_in,
   // Main memory interface (to DRAM/AXI)
   input  logic          mem_resp_valid,
   input  logic [255:0]  mem_resp_data,
@@ -20,10 +21,8 @@ module CachedCPU_RV64IMAFD_Zicsr_Zifencei_Microcoded_synth (
   CPU_RV64IMAFD_Zicsr_Zifencei_Microcoded_L1I256B_L1D256B_L2512B u_cpu (
     .clock(clock),
     .reset(reset),
-    .zero(1'b0),
-    .one(1'b1),
     .mem_resp_valid(mem_resp_valid),
-    .mtip_in(1'b0),
+    .mtip_in(mtip_in),
     .mem_resp_data(mem_resp_data),
     .mem_req_valid(mem_req_valid),
     .mem_req_addr(mem_req_addr),
